defined the logical relation

theories/examples/finelt/findom.v
@@ -3150,6 +3150,132 @@ Lemma app_respects : forall (f1 f2 : elt) (u1 u2 : elt),
 Proof.
 Admitted.
 
+
+  Definition is_bot (v : Valid.elt) : bool := 
+    match projT1 v with 
+    | Raw.bot => true
+    | _ => false
+    end.
+
+  Definition is_abs (v : Valid.elt) : option Valid.finfun := 
+    match v with 
+    | existT _ (Raw.abs e) Vf => Some (existT _ e Vf)
+    | _ => None
+    end.
+
+  Definition abs (f : finfun) : elt.
+    exists (Raw.abs (projT1 f)).
+    destruct f as [f Vf]. 
+    eassumption.
+  Defined.
+
+  Definition finfun_app (f : finfun) (u : elt) : elt.
+    destruct f as [f Vf].
+    destruct u as [u Vu].
+    destruct (Raw.app f u) eqn:h. 
+    { apply Raw.valid_app in h; eauto.
+      exists e. exact h. } 
+    { assert False.
+      destruct (Raw.valid_app_exists Vf Vu) as [w [Aw Vw]].
+      rewrite Aw in h. done. done. } 
+  Defined.
+
+  Definition graph (f : finfun) : list (elt * elt).
+    destruct f as [f Vf].
+    move: (Raw.valid_fun_subterms Vf) => h.
+    clear Vf.
+    move: h.
+    induction f as [|[u v]f].
+    move=> h. exact nil.
+    cbn.
+    move=> /andP.
+    move=> [/andP h1 h2]. 
+    eapply cons. destruct h1 as [Vu Vv].
+    eapply ((existT _ u Vu),(existT _ v Vv)).
+    eapply IHf; eauto.
+  Defined.
+
+  Definition compatible_fun (f g : finfun) : bool := 
+    Raw.compatible_fun (projT1 f) (projT1 g).
+
+  Definition coherent_with (f:finfun) : elt * elt -> bool := 
+    fun '(u, v) => 
+    Raw.coherent_with (projT1 f) (projT1 u, projT1 v).
+
+  Lemma In_graph_def (f : finfun) ui vi : 
+    In (projT1 ui, projT1 vi) (projT1 f) <->
+    In (ui, vi) (graph f).
+  Proof.
+    split.
+    + destruct f as [rf Vf]. move: Vf.
+      induction rf as [|[uj vj]f].
+      all: move=> Vf.
+      all: cbn [projT1].
+    - move=> h. inversion h.
+    - cbn [projT1] in IHf.
+      move=> [EQ|h].
+  Admitted.
+
+
+  Lemma coherent_with_def f u v :
+    (forallb 
+      (fun '(uj, vj) => compatible u uj ==> compatible v vj) (graph f)) <->
+    coherent_with f (u,v).
+  Proof.
+    split.
+    - move=> /forallb_forall CF. 
+      apply /forallb_forall.
+      move=> [rui rvi] Inrf.
+      have [ui E1]: { UI : elt & projT1 UI = rui }. 
+      { destruct f as [rf Vf]. cbn in Inrf.
+        have Vui: Raw.valid rui.
+        move: (Raw.valid_fun_subterms Vf) => /forallb_forall VSt.
+        specialize (VSt _ Inrf). cbn in VSt. 
+        move: VSt=> /andP. eauto.
+        exists (existT _ rui Vui). eauto. } 
+      have [vi E2]: { VI : elt & projT1 VI = rvi }. 
+      { destruct f as [rf Vf]. cbn in Inrf.
+        have Vvi: Raw.valid rvi.
+        move: (Raw.valid_fun_subterms Vf) => /forallb_forall VSt.
+        specialize (VSt _ Inrf). cbn in VSt. 
+        move: VSt=> /andP. eauto.
+        exists (existT _ rvi Vvi). eauto. } 
+      rewrite <- E1 in Inrf. rewrite <- E2 in Inrf.
+      rewrite In_graph_def in Inrf.
+      specialize (CF _ Inrf). cbn in CF. 
+      destruct ui. destruct vi. unfold compatible in CF.
+        cbn in CF. cbn in E1. cbn in E2. subst. done. 
+    - move=> /forallb_forall CF. 
+      apply /forallb_forall.
+      move=> [ui vi] Ingf.
+      rewrite <- In_graph_def in Ingf.
+      destruct ui. destruct vi. cbn in Ingf.
+      specialize (CF _ Ingf).
+      unfold compatible. cbn. eapply CF.
+  Qed.
+
+  Lemma compatible_fun_def (f g : finfun) : 
+    forallb (coherent_with g) (graph f) <-> 
+    compatible_fun f g.
+  Proof.
+    split.
+    - move=> /forallb_forall h.
+      unfold compatible_fun, Raw.compatible_fun.
+      apply /forallb_forall.
+      move=> [ui vi] Inf.
+  Admitted.
+
+  Lemma le_fun_mono_arg f u1 u2 :
+    le u1 u2 -> le (app f u1) (app f u2).
+  Proof.
+    move=> LE.
+    destruct f as [f Vf].
+    destruct u1 as [u1 Vu1].
+    destruct u2 as [u2 Vu2].
+    unfold le in LE. cbn [projT1] in LE. 
+  Admitted.
+
+
 End Valid.
 
 #[export] Instance eq_elt_equivalence : Equivalence Valid.eqb.
