theories/examples/finelt/raw_semantics.v
@@ -521,3 +521,4 @@ Lemma EvalRel_ideal {n} (M : Tm (S n)) ρ x1 x2 y1 y2 :
   eapply EvalRel_valid; eauto.
   eapply EvalRel_compatible; eauto.
 Qed.
+
