theories/examples/finelt/typing_semantics.v
@@ -1,0 +1,191 @@
+(* See LemmaForTS.agda/TypingSemantics.agda *)
+
+(* Prove that well typed syntax produces well typed interpretations
+
+i.e.  
+
+G |- M : A and fits G ρ implies
+
+    exists u a s.t. u : a, where [[M]]ρ = u and [[A]]ρ = a and 
+
+G |- M = N : A and fits G ρ implies 
+
+    exists u a s.t. u : a, where [[M]]ρ = u = [[N]]ρ
+
+ *)
+
+From Stdlib Require Import Relations List Program
+     ssreflect ssrfun ssrbool.
+From Stdlib Require Import Classes.RelationClasses 
+  Classes.Morphisms Lia Arith.
+
+Set Implicit Arguments.
+Unset Strict Implicit.
+Unset Printing Implicit Defensive.
+
+Require Import syntax.syntax.
+Require Import syntax.typing.
+
+Require Import findom.
+Require Import types.
+Require Import raw_semantics.
+
+
+Import SyntaxNotations.
+Import SubstNotations.
+
+Open Scope syntax_scope.
+
+Import Raw.
+
+(*
+------------------------------------------------------------------------
+-- Part 1: Fits — well-typed finite environments
+------------------------------------------------------------------------
+*)
+
+(* Theorem 1 *)
+
+(*  ρ fits Γ if for all x : A in Γ we have 
+                [[A]]ρ in Type and ρ(x) in [[A]]ρ. *)
+
+
+
+Inductive fits : forall {n} (Γ:Ctx n) (ρ : Env n), Prop := 
+  | fits_empty : fits ctx_empty null
+  | fits_cons n (Γ : Ctx n) A ρ a u i : 
+       typing Γ A (Core.tuniv i) ->
+       EvalRel A ρ a ->
+       wt a (tuniv i) ->
+       wt u a ->
+       fits Γ ρ ->
+       fits (Γ ++ A) (u .: ρ).
+
+Lemma fits_ctx {n} (Γ : Ctx n)(ρ : Env n) :
+  fits Γ ρ -> ctx Γ.
+Proof.
+  induction 1; eauto using ctx.
+Qed.
+
+Lemma fits_var {n} (Γ : Ctx n)(ρ : Env n) :
+  fits Γ ρ -> 
+  forall x, 
+  exists a i, typing Γ (lookup x Γ) (Core.tuniv i) /\
+         EvalRel (lookup x Γ) ρ a /\
+         wt a (tuniv i) /\
+         wt (ρ x) a.
+Proof.
+  move=> h.
+  induction h. done.
+  auto_case.
+  + destruct (IHh f) as [b [j [Ht [E [WT1 WT2]]]]].
+    exists b. exists j.
+    repeat split; auto.
+    eapply renaming_typing with (A := Core.tuniv j); 
+      eauto with renaming.
+    eapply c_cons; eauto using typing_ctx.
+    (* need a renaming lemma for EvalRel *)
+    (* 
+    E : EvalRel A ρ b
+    ============================
+    EvalRel (⟨↑⟩ A) (u .: ρ) b
+     *)
+    admit.
+Admitted.
+
+
+Lemma fits_tail {n} (Γ : Ctx n) (ρ : Env n) A u : 
+  fits (Γ ++ A) (u .: ρ) -> fits Γ ρ.
+move=> h. dependent destruction h; eauto.
+Admitted.
+
+Lemma fits_valid_env {n} (Γ : Ctx n)(ρ : Env n) :
+  fits Γ ρ -> valid_env ρ.
+Proof.
+  induction 1.
+  eapply valid_nil.
+  eapply valid_cons; eauto.
+  eapply wt_valid_tm; eauto.
+Qed.
+
+Hint Resolve fits_valid_env : valid typing.
+
+Lemma wt_bot_inv u : wt u bot -> u = bot.
+Proof. move=> h. inversion h. done. Qed. 
+
+Lemma wt_down u a : wt u a -> forall u', le u' u -> wt u' a.
+Proof.
+  move=> h. induction h.
+  all: move=> u' LE.
+  all: destruct u'; try done.
+  all: try solve [eapply wt_bot; eauto].
+  - cbn in LE. apply Nat.eqb_eq in LE. subst.
+    eapply wt_tuniv; eauto.
+  - eapply wt_tnat.
+  - eapply wt_zero.
+  - rewrite le_succ in LE.  eapply wt_succ; eauto.
+  - rewrite le_tpi in LE. move: LE => /andP. move=> [h1 h2].
+    eapply wt_tpi; eauto.
+    + move=> ui vi Inl.
+  (* SCW: I don't know how to finish the proof at this 
+     point, but I do need this for the theorem below *)
+Admitted.
+
+(*
+------------------------------------------------------------------------
+-- Part 2: Named invariants
+------------------------------------------------------------------------
+*)
+
+(* Typed M A rho u : 
+    exists u' = ⟦M⟧ρ and  u ≤ u' and exists a with u' : a and ⟦A⟧ρ = a
+*)
+Definition Typed {n:nat} (M : Tm n) (A : Tm n) ρ u := 
+  exists u' , exists a', 
+    le u u' /\ EvalRel M ρ u' /\ wt u' a' /\ EvalRel A ρ a'.
+
+(* InvTyp G M A rho : for all u ≤ ⟦M⟧ρ, Typed M A rho u *)
+Definition InvTyped 
+  {n:nat} (Γ: Ctx n) (M : Tm n) (A : Tm n) (ρ : Env n) := 
+  forall u, EvalRel M ρ u -> Typed M A ρ u.
+
+
+(* InvConv G M N A rho : typing for both + bidirectional evaluation *)
+Definition InvConv
+  {n:nat} (Γ: Ctx n) (M : Tm n) (N: Tm n) (A : Tm n) (ρ : Env n) := 
+  InvTyped Γ M A ρ 
+  /\ InvTyped Γ N A ρ 
+  /\ (forall u, EvalRel M ρ u -> EvalRel N ρ u) 
+  /\ (forall u, EvalRel N ρ u -> EvalRel M ρ u). 
+
+(*
+theorem1 : {n : Nat} {G : Ctx n} {M A : Expr n} ->
+    HasType G M A ->
+    (rho : EnvApprox n) -> Fits G rho ->
+    InvTyp G M A rho
+*)
+
+Fixpoint typing_EvalRel {n} (Γ : Ctx n) (M : Tm n) (A : Tm n) 
+   (h : typing Γ M A) {struct h} :
+   forall ρ, fits Γ ρ -> InvTyped Γ M A ρ
+with conv_EvalRel {n} (Γ : Ctx n) (M N : Tm n) (A : Tm n) 
+   (h : conv Γ M N A) {struct h} :
+  forall ρ, fits Γ ρ -> InvConv Γ M N A ρ.
+Proof.
+  - dependent destruction h.
+    all: move=> ρ Fρ.
+    + (* var *)
+      unfold InvTyped, Typed.
+      move=> u E.
+      move: E => [Vu Lu].
+      move: (fits_var Fρ x) => [a [i [hT [Ea [WT1 WT2]]]]].
+      exists u. exists a.
+      repeat split; 
+      eauto using le_refl, EvalRel_valid with valid.
+      eapply wt_down; eauto.
+    + eapply typing_EvalRel with (ρ:=ρ) in h; eauto.
+      eapply conv_EvalRel with (ρ:=ρ) in H; eauto.
+      move: H => [h1 [h2 [h3 h4]]].
+      move=> u EM.
+      admit.
+Admitted.
